theories/RocqsheetCofix.v
@@ -61,6 +61,7 @@ Definition trans (st : State) : State + option Z :=
         | CEmpty   => inl (mkSt (st_sheet st) (PCApply (Some 0%Z)) (st_stack st))
         | CLit n   => inl (mkSt (st_sheet st) (PCApply (Some n)) (st_stack st))
         | CFloat _ => inr None  (* cofix evaluator covers Z only *)
+        | CStr _   => inr None
         | CForm e' => inl (mkSt (st_sheet st)
                                 (PCEval (r :: visited) e') (st_stack st))
         end
@@ -134,6 +135,10 @@ Definition trans (st : State) : State + option Z :=
   | PCEval _ (EFSub _ _) => inr None
   | PCEval _ (EFMul _ _) => inr None
   | PCEval _ (EFDiv _ _) => inr None
+  | PCEval _ (EStr _) => inr None
+  | PCEval _ (EConcat _ _) => inr None
+  | PCEval _ (ELen _) => inr None
+  | PCEval _ (ESubstr _ _ _) => inr None
   | PCSumStep visited lc hc col row hr acc =>
       if PrimInt63.ltb hr row then
         inl (mkSt (st_sheet st) (PCApply (Some acc)) (st_stack st))
@@ -248,6 +253,7 @@ Definition eval_cell_co (s : Sheet) (r : CellRef) : itree NoE (option Z) :=
   | CEmpty   => Ret (Some 0%Z)
   | CLit n   => Ret (Some n)
   | CFloat _ => Ret None  (* cofix evaluator covers Z only *)
+  | CStr _   => Ret None
   | CForm e  => eval_co (r :: nil) s e
   end.
 
